Rename to RegExp.lean

ES2023/RegExp.lean
@@ -1,40 +1,80 @@
-import ES2023.RegExp.Def
+universe u
+
+/-- https://en.wikipedia.org/wiki/Regular_language#Formal_definition
+`α` is the type of alphabet allowed in the regular language. We make it universe-polymorphic. -/
+inductive RegExp (α: Type u)
+  /-- Matches nothing. -/
+  | nothing
+  /-- Empty string matcher. -/
+  | empty
+  | single (a: α)
+  /-- `/ab/` -/
+  | append (r₁ r₂: RegExp α)
+  /-- `/a|b/`-/
+  | union (r₁ r₂: RegExp α)
+  | star (r: RegExp α)
 
 namespace RegExp
-universe u
 variable {α : Type u}
 
-section
+/-
+Define convenient notations for `RegExp`.
+-/
+
+instance : EmptyCollection (RegExp α) where
+  emptyCollection := empty
+
+instance : Singleton α (RegExp α) where
+  singleton := single
+
+/-- Write `r ++ r'` for `RegExp.append r r'`. -/
+instance : Append (RegExp α) where
+  append := append
+
+/-- Write `r ∪ r'` for `RegExp.union r r'`. -/
+instance : Union (RegExp α) where
+  union := union
+
+/-- Write `r*` for `RegExp.star r`. This postfix operator `*` binds tighter
+than function application. -/
+postfix:arg "*" => star
+
+/-- Denoted by the Haskell operator `=~` to avoid overloading `∈` as done in
+theoretical computer science; really, `∈` is way too overloaded in math. We
+depart slightly from standard practice in that we do not require the type `α`
+to be finite. This results in a somewhat different theory of regular
+expressions, but the difference doesn't concern us here. -/
+inductive Accept: List α → RegExp α → Prop
+  | empty: Accept [] {}
+  | single {a: α}: Accept [a] {a}
+  | append {s₁ r₁ s₂ r₂}
+    : Accept s₁ r₁ → Accept s₂ r₂ → Accept (s₁ ++ s₂) (r₁ ++ r₂)
+  | unionL {s₁ r₁ r₂}: Accept s₁ r₁ → Accept s₁ (r₁ ∪ r₂)
+  | unionR {r₁ s₂ r₂}: Accept s₂ r₂ → Accept s₂ (r₁ ∪ r₂)
+  | starEmpty {r}: Accept [] r*
+  | starAppend {s₁ s₂ r}: Accept s₁ r → Accept s₂ r* → Accept (s₁ ++ s₂) r*
+
+@[inherit_doc] infix:50 " =~ " => Accept
+
+namespace Accept
 variable {a b : α} {s : List α} {r r₁ r₂ : RegExp α}
 
-theorem accept.nothing_def : ¬ s =~ nothing :=  (nomatch ·)
+theorem nothing_def : ¬ s =~ nothing :=  (nomatch ·)
 
-theorem accept.empty_def : s =~ {} → s = []
+theorem empty_def : s =~ {} → s = []
   | empty => rfl
 
-theorem accept.single_def : s =~ {a} → s = [a]
+theorem single_def : s =~ {a} → s = [a]
   | single => rfl
 
-example : a::s =~ {b} → a = b
-  | h => match h.single_def with | rfl => rfl
-
-example : a::s =~ {b} → s = []
-  | h => match h.single_def with | rfl => rfl
-
-example : s =~ nothing* → s = []
-  | .starEmpty => rfl
-
-example : s =~ r → s =~ r*
-  | h => s.append_nil ▸ h.starAppend .starEmpty
-
-theorem accept.app_exists : s =~ r₁ ++ r₂ → ∃ s₁ s₂, s = s₁ ++ s₂ ∧ s₁ =~ r₁ ∧ s₂ =~ r₂
+theorem app_exists : s =~ r₁ ++ r₂ → ∃ s₁ s₂, s = s₁ ++ s₂ ∧ s₁ =~ r₁ ∧ s₂ =~ r₂
   | append h₁ h₂ => ⟨_, _, rfl, h₁, h₂⟩
 
-theorem accept.union_disj : s =~ r₁ ∪ r₂ → s =~ r₁ ∨ s =~ r₂
+theorem union_disj : s =~ r₁ ∪ r₂ → s =~ r₁ ∨ s =~ r₂
   | unionL h => .inl h
   | unionR h => .inr h
 
-theorem accept.cons_append
+theorem cons_append
   : a::s =~ r₁ ++ r₂
   → (∃ s₁ s₂, s = s₁ ++ s₂ ∧ a::s₁ =~ r₁ ∧ s₂ =~ r₂) ∨
     ([] =~ r₁ ∧ a::s =~ r₂)
@@ -45,10 +85,39 @@ theorem accept.cons_append
   | .append (s₁ := b::s₁) h₁ h₂ =>
     cases et; exact .inl ⟨_, _, rfl, h₁, h₂⟩
 
+theorem starRec {motive : ∀ {s}, s =~ r* → Prop}
+  (base : motive .starEmpty)
+  (ind : ∀ {s₁ s₂}, (h₁ : s₁ =~ r) → (h₂ : s₂ =~ r*)
+    → motive h₂ → motive (h₁.starAppend h₂))
+  {s} (h : s =~ r*) : motive h
+:= by
+  generalize er : r* = r; rw [er] at h
+  induction h
+  case empty | single | append | unionL | unionR => exact nomatch er
+  case starEmpty => exact base
+  case starAppend s₁ s₂ _ h₁ h₂ _ ih =>
+    cases er; cases s₁
+    . case nil => exact ih h rfl
+    . case cons => exact ind h₁ h₂ (ih h₂ rfl)
+
+theorem cons_star
+  : a::s =~ r* → ∃ s₁ s₂, s = s₁ ++ s₂ ∧ a::s₁ =~ r ∧ s₂ =~ r*
+:= by
+  generalize et : a::s = t
+  intros h
+  induction h using starRec
+  case base => exact nomatch et
+  case ind s₁ s₂ h₁ h₂ ih =>
+    cases s₁
+    . case nil => exact ih et
+    . case cons => cases et; exact ⟨_, _, rfl, h₁, h₂⟩
+
+end Accept
+
 instance match_empty : (r : RegExp α) → Decidable ([] =~ r)
-  | nothing => isFalse accept.nothing_def
+  | nothing => isFalse Accept.nothing_def
   | empty => isTrue .empty
-  | single _ => isFalse (nomatch accept.single_def ·)
+  | single _ => isFalse (nomatch Accept.single_def ·)
   | append r₁ r₂ =>
     match match_empty r₁, match_empty r₂ with
     | isTrue h₁, isTrue h₂ => isTrue (h₁.append h₂)
@@ -65,35 +134,6 @@ instance match_empty : (r : RegExp α) → Decidable ([] =~ r)
     | _, isTrue h => isTrue h.unionR
   | _* => isTrue .starEmpty
 
-theorem accept.starRec {motive : ∀ {s}, s =~ r* → Prop}
-  (base : motive .starEmpty)
-  (ind : ∀ {s₁ s₂}, (h₁ : s₁ =~ r) → (h₂ : s₂ =~ r*)
-    → motive h₂ → motive (h₁.starAppend h₂))
-  {s} (h : s =~ r*) : motive h
-:= by
-  generalize er : r* = r; rw [er] at h
-  induction h
-  case empty | single | append | unionL | unionR => exact nomatch er
-  case starEmpty => exact base
-  case starAppend s₁ s₂ _ h₁ h₂ _ ih =>
-    cases er; cases s₁
-    . case nil => exact ih h rfl
-    . case cons => exact ind h₁ h₂ (ih h₂ rfl)
-
-theorem accept.cons_star
-  : a::s =~ r* → ∃ s₁ s₂, s = s₁ ++ s₂ ∧ a::s₁ =~ r ∧ s₂ =~ r*
-:= by
-  generalize et : a::s = t
-  intros h
-  induction h using accept.starRec
-  case base => exact nomatch et
-  case ind s₁ s₂ h₁ h₂ ih =>
-    cases s₁
-    . case nil => exact ih et
-    . case cons => cases et; exact ⟨_, _, rfl, h₁, h₂⟩
-
-end
-
 section
 variable [DecidableEq α]
 
@@ -109,7 +149,7 @@ def derive (a : α) : RegExp α → RegExp α
   | union r₁ r₂ => derive a r₁ ∪ derive a r₂
   | r* => derive a r ++ r*
 
-theorem accept.cons_derive {a} {s : List α} : {r : RegExp α} → a::s =~ r → s =~ derive a r
+theorem Accept.cons_derive {a} {s : List α} : {r : RegExp α} → a::s =~ r → s =~ derive a r
   | nothing, h => h.nothing_def.rec
   | .empty, h => nomatch h.empty_def
   | .single _, h => match h.single_def.symm with | rfl => trans empty (if_pos rfl).symm
@@ -122,7 +162,7 @@ theorem accept.cons_derive {a} {s : List α} : {r : RegExp α} → a::s =~ r →
   | union .., h => h.union_disj.rec (unionL ∘ cons_derive) (unionR ∘ cons_derive)
   | _*, h => have ⟨_, _, h, h₁, h₂⟩ := h.cons_star ; h ▸ h₁.cons_derive.append h₂
 
-theorem accept.derive_cons {a} {s : List α} : {r : RegExp α} → s =~ derive a r → a::s =~ r
+theorem Accept.derive_cons {a} {s : List α} : {r : RegExp α} → s =~ derive a r → a::s =~ r
   | .single b, h => if e : a = b
     then match trans h (if_pos e) with | empty => e ▸ single
     else nomatch trans h (if_neg e)
